src/asn1/ASN1.Spec.OCTET_STRING.fst
@@ -8,28 +8,28 @@ open ASN1.Base
 open ASN1.Spec.Tag
 open ASN1.Spec.Length
 
-module I = FStar.Integers
+open FStar.Integers
 
 // let synth_asn1_octet_string
 //   (l: asn1_length_t)
 //   (ls: lbytes l)
-// : GTot (x: datatype_of_asn1_type OCTET_STRING{I.v (dfst x) == l})
+// : GTot (x: datatype_of_asn1_type OCTET_STRING{v (dfst x) == l})
 //   // (requires True)
-//   // (ensures fun x -> I.v (dfst x) == l)
+//   // (ensures fun x -> v (dfst x) == l)
 // = (|I.u l, ls|)
 
 // let synth_asn1_octet_string_inverse
 //   (l: asn1_length_t)
-//   (x: datatype_of_asn1_type OCTET_STRING{I.v (dfst x) == l})
+//   (x: datatype_of_asn1_type OCTET_STRING{v (dfst x) == l})
 // : GTot (ls: lbytes l)
-//   // (requires I.v (dfst x) == l)
+//   // (requires v (dfst x) == l)
 //   // (ensures fun ls -> synth_asn1_octet_string l ls == x)
 // = dsnd x
 
 let parse_asn1_octet_string_kind (l: asn1_length_t) = total_constant_size_parser_kind l
 let parse_asn1_octet_string
   (l: asn1_length_t)
-// : parser (parse_asn1_octet_string_kind l) (x: datatype_of_asn1_type OCTET_STRING{I.v (dfst x) == l})
+// : parser (parse_asn1_octet_string_kind l) (x: datatype_of_asn1_type OCTET_STRING{v (dfst x) == l})
 = parse_seq_flbytes l
 //   `parse_synth`
 //   synth_asn1_octet_string l
@@ -62,71 +62,76 @@ let serialize_asn1_octet_string_weak
 /// Specialized TLV
 ///
 // let synth_asn1_octet_string_L
-//   (x: the_asn1_type OCTET_STRING * asn1_len_of_tag OCTET_STRING)
+//   (x: the_asn1_type OCTET_STRING & asn1_len_of_tag OCTET_STRING)
 // : GTot (asn1_len_of_tag OCTET_STRING)
 // = snd x
 
 // let synth_asn1_octet_string_L_inverse
 //   (len: asn1_len_of_tag OCTET_STRING)
-// : GTot (x: (the_asn1_type OCTET_STRING * asn1_len_of_tag OCTET_STRING){len == synth_asn1_octet_string_L x})
+// : GTot (x: (the_asn1_type OCTET_STRING & asn1_len_of_tag OCTET_STRING){len == synth_asn1_octet_string_L x})
 // = (OCTET_STRING, len)
 
 let parser_tag_of_octet_string
   (x: datatype_of_asn1_type OCTET_STRING)
-: GTot (the_asn1_type OCTET_STRING * asn1_int32_of_tag OCTET_STRING)
+: GTot (the_asn1_type OCTET_STRING & asn1_int32_of_tag OCTET_STRING)
 = (OCTET_STRING, dfst x)
 
-let synth_asn1_octet_string_V
+let synth_asn1_octet_string_data
   (len: asn1_int32_of_tag OCTET_STRING)
-  (x: the_asn1_type OCTET_STRING * asn1_int32_of_tag OCTET_STRING{x == (OCTET_STRING, len)})
-  (s: lbytes (I.v len))
+  (x: the_asn1_type OCTET_STRING & asn1_int32_of_tag OCTET_STRING{x == (OCTET_STRING, len)})
+  (s: lbytes (v len))
 : GTot (refine_with_tag parser_tag_of_octet_string x)
 = let value: datatype_of_asn1_type OCTET_STRING = (|len, s|) in
   let y: refine_with_tag parser_tag_of_octet_string x = value in
   y
 
-let synth_asn1_octet_string_V_inverse
+let synth_asn1_octet_string_data_inverse
   (len: asn1_int32_of_tag OCTET_STRING)
-  (x: the_asn1_type OCTET_STRING * asn1_int32_of_tag OCTET_STRING{x == (OCTET_STRING, len)})
+  (x: the_asn1_type OCTET_STRING & asn1_int32_of_tag OCTET_STRING{x == (OCTET_STRING, len)})
   (value: refine_with_tag parser_tag_of_octet_string x)
-: GTot (s: lbytes (I.v len))
+: GTot (s: lbytes (v len))
 = dsnd
-    #asn1_int32
-    #(fun (len:asn1_int32) -> s:bytes{Seq.length s == I.v len})
+    #(asn1_int32_of_tag OCTET_STRING)
+    #(fun (len:asn1_int32_of_tag OCTET_STRING) -> s:bytes{Seq.length s == v len})
     value
 
 let parse_asn1_octet_string_kind_strong
-  (x: the_asn1_type OCTET_STRING * asn1_int32_of_tag OCTET_STRING)
+  (x: the_asn1_type OCTET_STRING & asn1_int32_of_tag OCTET_STRING)
 : parser_kind
-= total_constant_size_parser_kind (I.v (snd x))
+= total_constant_size_parser_kind (v (snd x))
 
 let parse_asn1_octet_string_data
-  (x: the_asn1_type OCTET_STRING * asn1_int32_of_tag OCTET_STRING)
+  (x: the_asn1_type OCTET_STRING & asn1_int32_of_tag OCTET_STRING)
 : Tot (parser (parse_asn1_octet_string_kind_strong x) (refine_with_tag parser_tag_of_octet_string x))
-= parse_asn1_octet_string (I.v (snd x))
+= parse_asn1_octet_string (v (snd x))
   `parse_synth`
-  synth_asn1_octet_string_V (snd x) x
+  synth_asn1_octet_string_data (snd x) x
 
+let parse_asn1_octet_string_data_unfold
+  (input: bytes)
+: Lemma (
+  forall (x: the_asn1_type OCTET_STRING & asn1_int32_of_tag OCTET_STRING).
+)
 
 let serialize_asn1_octet_string_data
-  (x: the_asn1_type OCTET_STRING * asn1_int32_of_tag OCTET_STRING)
+  (x: the_asn1_type OCTET_STRING & asn1_int32_of_tag OCTET_STRING)
 : Tot (serializer (parse_asn1_octet_string_data x))
 = serialize_synth
-  (* p1 *) (parse_asn1_octet_string (I.v (snd x)))
-  (* f2 *) (synth_asn1_octet_string_V (snd x) x)
-  (* s1 *) (serialize_asn1_octet_string (I.v (snd x)))
-  (* g1 *) (synth_asn1_octet_string_V_inverse (snd x) x)
+  (* p1 *) (parse_asn1_octet_string (v (snd x)))
+  (* f2 *) (synth_asn1_octet_string_data (snd x) x)
+  (* s1 *) (serialize_asn1_octet_string (v (snd x)))
+  (* g1 *) (synth_asn1_octet_string_data_inverse (snd x) x)
   (* Prf*) ()
 
 let parse_asn1_octet_string_data_weak
-  (x: the_asn1_type OCTET_STRING * asn1_int32_of_tag OCTET_STRING)
+  (x: the_asn1_type OCTET_STRING & asn1_int32_of_tag OCTET_STRING)
 : Tot (parser parse_asn1_octet_string_kind_weak (refine_with_tag parser_tag_of_octet_string x))
 = parse_asn1_octet_string_kind_weak
   `weaken`
   parse_asn1_octet_string_data x
 
 let serialize_asn1_octet_string_data_weak
-  (x: the_asn1_type OCTET_STRING * asn1_int32_of_tag OCTET_STRING)
+  (x: the_asn1_type OCTET_STRING & asn1_int32_of_tag OCTET_STRING)
 : Tot (serializer (parse_asn1_octet_string_data_weak x))
 = parse_asn1_octet_string_kind_weak
   `serialize_weaken`
@@ -156,6 +161,32 @@ let parse_asn1_octet_string_TLV
   (* tg *) (parser_tag_of_octet_string)
   (* p  *) (parse_asn1_octet_string_data_weak)
 
+let parse_asn1_octet_string_TLV_unfold
+  (input: bytes)
+: Lemma (
+  parse parse_asn1_octet_string_TLV input ==
+ (match parse (parse_the_asn1_tag OCTET_STRING) input with
+  | None -> None
+  | Some (v_T, l_T) ->
+    (let input_LV = Seq.slice input l_T (Seq.length input) in
+     match parse (parse_asn1_length_of_tag OCTET_STRING) input_LV with
+     | None -> None
+     | Some (v_L, l_L) ->
+       (let input_data = Seq.slice input_LV l_L (Seq.length input_LV) in
+        match parse (parse_asn1_octet_string_data (v_T, v_L)) input_data with
+        | None -> None
+        | Some (v_V, l_V) -> Some (v_V, (l_T + l_L + l_V <: consumed_length input)))
+     ))
+)
+= nondep_then_eq
+  (* p1 *) (parse_the_asn1_tag OCTET_STRING)
+  (* p2 *) (parse_asn1_length_of_tag OCTET_STRING)
+  (* in *) (input);
+  parse_synth_eq
+  (* p1 *) (parse_asn1_octet_string (v (snd x)))
+  (* f2 *) (synth_asn1_octet_string_data)
+  (* in *)
+
 let serialize_asn1_octet_string_TLV
 : serializer parse_asn1_octet_string_TLV
 = serialize_tagged_union
@@ -165,3 +196,12 @@ let serialize_asn1_octet_string_TLV
   (* tg *) (parser_tag_of_octet_string)
   (* s  *) (serialize_asn1_octet_string_data_weak)
 
+let length_lemma
+  (input: bytes)
+: Lemma
+  (requires (Some? (parse parse_asn1_octet_string_TLV input)))
+  (ensures (
+    let px = parse parse_asn1_octet_string_TLV input in
+    let pt = parse (parse_the_asn1_tag OCTET_STRING) input in
+    let pl = parse (parse_asn1_length_of_tag OCTET_STRING) (Seq.slice input 0 )
+  ))
